Only allow contracts access to their own balance (#82)
Remove the account_balance function from Chain and add instead
ctx_contract_balance to the ContractCallContext. This is is the only
thing our contracts use and it means that we match the models of our
target languages better. It also means we do not need Proper instances
anymore for contracts.

execution/theories/Circulation.v
@@ -10,8 +10,8 @@ Context {ChainBase : ChainBase}.
 Context `{Finite Address}.
 
 Local Open Scope Z.
-Definition circulation (chain : Chain) :=
-  sumZ (account_balance chain) (elements Address).
+Definition circulation (env : Environment) :=
+  sumZ (env_account_balances env) (elements Address).
 
 (* We prove first that over any single action, the circulation is preserved.
 The idea behind this proof is that addrs contain from and to so
@@ -69,7 +69,8 @@ Proof.
   cbn.
   rewrite (account_balance_post_to eval from_neq_to).
   rewrite (account_balance_post_from eval from_neq_to).
-  enough (sumZ (account_balance pre) suf = sumZ (account_balance post) suf) by lia.
+  enough (sumZ (env_account_balances pre) suf = sumZ (env_account_balances post) suf)
+    by lia.
 
   pose proof (Permutation_NoDup perm) as perm_set.
   assert (from_not_in_suf: ~In (eval_from eval) suf).
@@ -87,10 +88,10 @@ Qed.
 Hint Resolve eval_action_circulation_unchanged : core.
 
 Instance circulation_proper :
-  Proper (ChainEquiv ==> eq) circulation.
+  Proper (EnvironmentEquiv ==> eq) circulation.
 Proof.
   intros x y [].
-  unfold circulation, account_balance.
+  unfold circulation, env_account_balances.
   induction (elements Address) as [|z zs IH]; auto.
   cbn.
   now
@@ -99,6 +100,7 @@ Proof.
     | [H: _ |- _] => rewrite H
   end.
 Qed.
+
 
 (* Now we prove that adding a block _does_ increase the circulation
 by what we would expect. *)
